# 1. Show that $\a + \b = \b + \a \quad \forall \a, \b \in \C$.
  Suppose $\alpha = a+bi$  and $\beta = c+di$,where $a,b,c,d \in \R$. 
  The [[1. Real space and Complex Space#^881fa0|definition of complex numbers]] show that:$$\begin{align}\a+\b &= (a+bi)+(c+di)\\ &=(a+c)+(b+d)i\end{align} \tag1$$and$$\begin{align}\b+\a &= (c+di)+(a+bi)\\ &=(c+a)+(d+b)i\end{align} \tag2$$ From $(1)$ and $(2) \implies \a+\b = \b+\a$, $\forall \a, \b \in \C$
# 2. Show that $(\a + \b) + \ld = \a + (\b +\ld) \quad \forall \a,\b,\ld \in \C$
  Suppose $\a = a+bi$, $\b=c +di$ and $\ld = e +fi$, where $a,b,c,d,e,f \in \R$. The [[1. Real space and Complex Space#^881fa0|definition of complex numbers]] show that $$(\a+\b)+\ld =(a+c+e)+(b+d+f)i \tag3$$and$$\a+(\b+\ld)=(a+c+e)+(b+d+f)i\tag4$$From $(3)$ and $(4) \implies (\a +\b)+\ld=\a+(\b+\ld)$, $\forall \a,\b,\ld \in \C$
# 3. Show that $(\a \b)\ld = \a(\b \ld) \quad \forall \a, \b, \ld \in C$
Suppose $\a = a+bi$, $\b=c +di$ and $\ld = e +fi$, where $a,b,c,d,e,f \in \R$. The [[1. Real space and Complex Space#^881fa0|definition of complex numbers]] show that $$(\a \b)\ld = (ace-bde-adf-bcf)+(ade+bce+acf-bdf)i\tag 5$$and$$\a(\b\ld) = (ace-bde-adf-bcf)+(ade+bce+acf-bdf)i \tag 6$$From $(5)$ and $(6) \implies (\a\b)\ld = \a(\b\ld)$, $\forall \a, \b, \ld \in \C$
# 4. Show that $\ld (\a + \b) = \ld \a + \ld \b \quad \forall \ld, \a, \b \in C$
 Suppose $\a = a+bi$, $\b=c +di$ and $\ld = e +fi$, where $a,b,c,d,e,f \in \R$. The [[1. Real space and Complex Space#^881fa0|definition of complex numbers]] show that:$$\begin{align}\ld(\a + \b) &= (e+fi)\big((a+c)+(b+d)i\big)\\ & = (ae+ce -fb -fd)+(af+cf+eb+ed)i\end{align} \tag {7}$$and$$\begin{align}\ld \a + \ld \b &= (e+fi)(a+bi)+(e+fi)(c+di) \\ &= (ae+ce-fb-fd)+(af+cf+eb+ed)i\end{align} \tag{8}$$From $(7)$ and $(8) \implies \ld(\a+\b) = \ld \a + \ld \b$, $\forall \ld, \a, \b \in \C$
# 5. Show that for every $\a \in \C, \quad \exists! \b \in \C: \a + \b = 0$   
  Suppose there exist $\b, \ld \in \C$ such that $\a+\b = 0$ and $\a + \ld = 0$, so with [[#^12d8d0|identity property]], we have:$$\b = \b + 0 = \b + (a+\b) = \b + (\a+ \ld)$$ With commutativity and [[#^10ce7f|associativity]] properties, we have: $$\b + (\a +\ld) = (\b +\a) + \ld = \ld + 0 = \ld$$ So $\b = \ld \implies$ for every $\a \in \C$, there is a unique $\b \in \C$ such that $\a +\b =0$
# 6. Show that $\forall \a \in \C \text{ with } \a \not = 0, \exists ! \b \in \C$ 
 Suppose $\b = \frac 1 \a$, because $\a \not = 0$, we have:
 $$
 \begin{align}
 \a \b = \a \cdot \frac 1 \a = 1
 \end{align}
$$
Suppose there is $\b_1$ and $\b_2 \in \C$
$$
\begin{aligned}
&\a \b_1 = 1 \\
&\a \b_2 = 1 \\
&\implies \a \b_1 - \a\b_2 = 0 \\
&\iff \b_1 - \b_2 = 0 \text{ (since } \a \not = 0 ) \\
&\iff \b_1 = \b_2
\end{aligned}
$$
# 7. Show that $$\frac{-1+\sqrt3 i}{2}$$ is a cube root of 1.
$$
\begin{align}
A &= \frac{-1+\sqrt3 i}{2} \cdot \frac{-1+\sqrt3 i}{2} \cdot \frac{-1+\sqrt3 i}{2} \\
&= \frac{(\sqrt3 i -1)^2}{4}\cdot\frac{-1+\sqrt3 i}{2} \\
&= \frac {-3-2\sqrt{3}i +1}{4} \cdot \frac{-1+\sqrt3 i}{2} \\
&= \frac{-1-\sqrt3 i}{2} \cdot \frac{-1+\sqrt3 i}{2} \\
&= \frac{1-\sqrt3 i + \sqrt3i+3}{4} = 1
\end{align}
$$
# 8. Find two distinct square roots of $i$
Let's $z \in \C$ is the square roots of $i$:
$$
\begin{align}
i = z^2 &= (a+bi)^2 \\
&= a^2 - b^2 + 2abi \\
\end{align}
$$
// // // // // /// /// /// /// /// // /// / / / / / / / ///// / / /// // / / / //// //// /////