Bandit problems in which the reward probabilities do not change over time -> stationary problem.

If the problem is nonstationary, it make more sense to give more weight to recent rewards than the long-past rewards (see [[2. Random Forests]]).

Modifying the [[2.4 Incremental Implementation#^88f053| update rule for updating an average Q of the n-1 past rewards]] to be:
$$
\begin{align}
Q_{n+1} &= Q_n + \a[R_n - Q_n] \qquad \a \in (0,1] \\
& = \a R_n + (1-\a)Q_n \\
& = \a R_n + (1-\a)[\a R_{n-1} + (1-\a)Q_{n-1}] \\
& = \a R_n + (1-\a)\a R_{n-1} + (1-\a)^2Q_{n-1} \\
& = \a R_n + (1-\a)\a R_{n-1} + (1-\a)^2 [\a R_{n-2} + (1-\a)Q_{n-2}] \\
& = \a R_n + (1-\a)\a R_{n-1} + (1-\a)^2 \a R_{n-2} + (1-\a)^3Q_{n-2} \\
& \qquad \qquad \cdots \\
& = (1-\a)^n Q_1 + \sum_{i=1}^n \a(1-\a)^{n-i}R_i
\end{align}
$$

^a6519d

-> Weighted average sum. The weight: $(1-\a)^n + \sum_{i=1}^n \a(1-\a)^{n-i} = 1$   

Let $\a_n(a)$ denote the step-size parameter used to process the reward received after the $n$th selection of $a$. 

If $\a_n(a) = \frac 1 n$ -> [[2.4 Incremental Implementation#^a686db|sample-average method]] -> guaranteed to converge to the true action values by the law of large numbers.

Convergence is not guaranteed for all choices of the sequence ${\a_n(a)}$.

The conditions required to assure convergence with probability 1:
$$
\sum_{n=1}^{\infty} \a_n(a) = \infty \qquad \qquad \text {and} \qquad \qquad \sum_{n=1}^{\infty} \a^2_n(a) < \infty
$$
* The first condition is required to guarantee that the steps are large enough to eventually overcome any initial conditions or random fluctuations.
* The second condition guarantees that eventually the steps become small enough to assure convergence
-> slow af.

Ex 2.4:
$$
\begin{align}
Q_{n+1} &= Q_n + \a_n[R_n - Q_n] \\
& = \a_n R_n + (1-\a_n)Q_n \\
& = \a_n R_n + (1-\a_n) [\a_{n-1}R_{n-1} +  (1-\a_{n-1})Q_{n-1}] \\
& = \a_n R_n + (1-\a_n)\a_{n-1}R_{n-1} + (1-\a_n)(1-\a_{n-1})Q_{n-1} \\
& = \a_n R_n + (1-\a_n)\a_{n-1}R_{n-1} + (1-\a_n)(1-\a_{n-1})[\a_{n-2}R_{n-2} +  (1-\a_{n-2})Q_{n-2}] \\
& \dots \\
& = \sum_{i=1}^n \a_iR_i \prod_{j=i+1}^{n} (1-\a_j) + \prod_{i=1}^n (1-\a_i)Q_1
\end{align} \\
$$

$$

$$